minor changes. update to eiger-port refinement

txn-data-consistency/CCv_Eiger_Port_modified.thy
@@ -74,17 +74,17 @@ definition cls_svr_k'_t'_unchanged where
 definition svrs_cls_cl'_unchanged where
   "svrs_cls_cl'_unchanged cl s s' \<equiv> svrs s' = svrs s \<and> other_insts_unchanged cl (cls s) (cls s')"
 
-lemmas km_unchanged_defs = cls_svr_k'_t'_unchanged_def other_insts_unchanged_def svr_t'_unchanged_def
-lemmas tm_unchanged_defs = svrs_cls_cl'_unchanged_def other_insts_unchanged_def
-lemmas unchanged_defs = km_unchanged_defs svrs_cls_cl'_unchanged_def
+lemmas svr_unchanged_defs = cls_svr_k'_t'_unchanged_def other_insts_unchanged_def svr_t'_unchanged_def
+lemmas cl_unchanged_defs = svrs_cls_cl'_unchanged_def other_insts_unchanged_def
+lemmas unchanged_defs = svr_unchanged_defs svrs_cls_cl'_unchanged_def
 
 definition tid_match :: "'v state \<Rightarrow> txid0 \<Rightarrow> bool" where
   "tid_match s t \<equiv> txn_sn (cls s (get_cl_txn t)) = get_sn_txn t"
 
-abbreviation add_to_readerset :: "'v ep_version list \<Rightarrow> txid0 \<Rightarrow> v_id \<Rightarrow> 'v ep_version list" where
+definition add_to_readerset :: "'v ep_version list \<Rightarrow> txid0 \<Rightarrow> v_id \<Rightarrow> 'v ep_version list" where
   "add_to_readerset vl t i \<equiv> vl [i := (vl ! i)\<lparr>v_readerset := insert t (v_readerset (vl ! i))\<rparr>]"
 
-abbreviation commit_in_vl :: "'v ep_version list \<Rightarrow> tstmp \<Rightarrow> v_id \<Rightarrow> 'v ep_version list" where
+definition commit_in_vl :: "'v ep_version list \<Rightarrow> tstmp \<Rightarrow> v_id \<Rightarrow> 'v ep_version list" where
   "commit_in_vl vl commit_t i \<equiv> vl [i := (vl ! i)\<lparr>v_ts := commit_t, v_is_pending := False\<rparr>]"
 
 abbreviation get_txn_cl :: "'v state \<Rightarrow> cl_id \<Rightarrow> txid0" where
@@ -140,13 +140,13 @@ definition read :: "cl_id \<Rightarrow> key \<Rightarrow> 'v \<Rightarrow> 'v st
     svrs_cls_cl'_unchanged cl s s'"
 
 definition read_done :: "cl_id \<Rightarrow> (key \<rightharpoonup> 'v) \<Rightarrow> sqn \<Rightarrow> view \<Rightarrow> 'v state \<Rightarrow> 'v state \<Rightarrow> bool" where
-  "read_done cl kv_map sn u s s' \<equiv>
+  "read_done cl kv_map sn u'' s s' \<equiv>
     sn = txn_sn (cls s cl) \<and>
-    u = cl_view (cls s cl) \<and>
+    u'' = cl_view (cls s' cl) \<and>
     (\<forall>k \<in> dom kv_map. \<exists>v i.
      (v, i) = read_at (rev (DS (svrs s k))) (gst (cls s cl)) cl \<and>
      cl_view (cls s' cl) k = insert i (cl_view (cls s cl) k)) \<and>
-    (\<exists>keys. txn_state (cls s cl) = RtxnInProg keys kv_map \<and> dom kv_map = keys) \<and>
+    txn_state (cls s cl) = RtxnInProg (dom kv_map) kv_map \<and>
     txn_state (cls s' cl) = Idle \<and>
     txn_sn (cls s' cl) = Suc (txn_sn (cls s cl)) \<and>
     gst (cls s' cl) = gst (cls s cl) \<and>
@@ -284,21 +284,20 @@ lemma tps_trans [simp]: "trans tps = state_trans" by (simp add: tps_def)
 subsubsection \<open>Refinement\<close>
 
 \<comment> \<open>Simulation function\<close>
-abbreviation pending_rtxn :: "'v state \<Rightarrow> txid0 \<Rightarrow> bool" where
+definition pending_rtxn :: "'v state \<Rightarrow> txid0 \<Rightarrow> bool" where
   "pending_rtxn s t \<equiv> \<exists>keys kv_map. txn_state (cls s (get_cl_txn t)) = RtxnInProg keys kv_map \<and>
     txn_sn (cls s (get_cl_txn t)) = get_sn_txn t"
 
-abbreviation pending_wtxn :: "'v state \<Rightarrow> txid \<Rightarrow> bool" where
+definition pending_wtxn :: "'v state \<Rightarrow> txid \<Rightarrow> bool" where
   "pending_wtxn s t' \<equiv> case t' of T0 \<Rightarrow> False |
-    Tn t \<Rightarrow> \<exists>kv_map. txn_state (cls s (get_cl_txn t)) = WtxnPrep kv_map \<and>
-                txn_sn (cls s (get_cl_txn t)) = get_sn_txn t"
+    Tn (Tn_cl sn cl) \<Rightarrow> \<exists>kv_map. txn_state (cls s cl) = WtxnPrep kv_map \<and> txn_sn (cls s cl) = sn"
 
 definition get_ver_committed_rd :: "'v state \<Rightarrow> 'v ep_version \<Rightarrow> 'v version" where
   "get_ver_committed_rd s v \<equiv>
    \<lparr>v_value = v_value v, v_writer = v_writer v, v_readerset = v_readerset v - {t. pending_rtxn s t}\<rparr>"
 
 definition get_vl_committed_wr :: "'v state \<Rightarrow> 'v ep_version list \<Rightarrow> 'v ep_version list" where
-  "get_vl_committed_wr s vl \<equiv> filter (\<lambda>v. v_is_pending v \<and> pending_wtxn s (v_writer v)) vl"
+  "get_vl_committed_wr s vl \<equiv> filter (\<lambda>v. \<not>v_is_pending v \<or> \<not>pending_wtxn s (v_writer v)) vl"
 
 definition kvs_of_s :: "'v state \<Rightarrow> 'v kv_store" where
   "kvs_of_s s = (\<lambda>k. map (get_ver_committed_rd s) (get_vl_committed_wr s (DS (svrs s k))))"
@@ -310,10 +309,345 @@ definition sim :: "'v state \<Rightarrow> 'v config" where
   "sim s = (kvs_of_s s, views_of_s s)"
 
 lemmas sim_defs = sim_def kvs_of_s_def views_of_s_def
+lemmas get_state_defs = get_ver_committed_rd_def get_vl_committed_wr_def
 
 \<comment> \<open>Mediator function\<close>
 fun med :: "'v ev \<Rightarrow> 'v label" where
-  "med (RDone cl kv_map sn u) = ET cl sn u (\<lambda>k op. case op of R \<Rightarrow> kv_map k | W \<Rightarrow> None)" |
-  "med (WCommit cl kv_map _ sn u) = ET cl sn u (\<lambda>k op. case op of R \<Rightarrow> None | W \<Rightarrow> kv_map k)" |
+  "med (RDone cl kv_map sn u'') = ET cl sn u'' (\<lambda>k op. case op of R \<Rightarrow> kv_map k | W \<Rightarrow> None)" |
+  "med (WCommit cl kv_map _ sn u'') = ET cl sn u'' (\<lambda>k op. case op of R \<Rightarrow> None | W \<Rightarrow> kv_map k)" |
   "med _ = ETSkip"
 
+\<comment> \<open>lemmas for unchanged elements in svrs\<close>
+
+lemma DS_eq_all_k:
+  assumes "DS (svrs s' k) = DS (svrs s k)"
+    and "other_insts_unchanged k (svrs s) (svrs s')"
+  shows "\<forall>k. DS (svrs s' k) = DS (svrs s k)"
+  using assms by (auto simp add: other_insts_unchanged_def)
+
+lemma eq_for_all_k: 
+  assumes "f (svrs s' k) t = f (svrs s k) t"
+    and "\<forall>k'. k' \<noteq> k \<longrightarrow> svrs s' k' = svrs s k'"
+    and "\<forall>t'. t' \<noteq> t \<longrightarrow> f (svrs s' k) t' = f (svrs s k) t'"
+  shows "\<forall>k. f (svrs s' k) = f (svrs s k)"
+  apply (auto simp add: fun_eq_iff) using assms
+  subgoal for k' t' by (cases "k' = k"; cases "t' = t"; simp).
+
+lemma eq_for_all_cl:
+  assumes "f (cls s' cl) = f (cls s cl)"
+    and "\<forall>cl'. cl' \<noteq> cl \<longrightarrow> cls s' cl' = cls s cl'"
+  shows "\<forall>cl. f (cls s' cl) = f (cls s cl)"
+  apply (auto simp add: fun_eq_iff) using assms
+  subgoal for cl' by (cases "cl' = cl"; simp).
+
+\<comment> \<open>Invariants about kv store\<close>
+definition KVSNonEmp where
+  "KVSNonEmp s \<longleftrightarrow> (\<forall>k. DS (svrs s k) \<noteq> [])"
+
+lemmas KVSNonEmpI = KVSNonEmp_def[THEN iffD2, rule_format]
+lemmas KVSNonEmpE[elim] = KVSNonEmp_def[THEN iffD1, elim_format, rule_format]
+
+lemma reach_kvs_non_emp [simp, intro]: "reach tps s \<Longrightarrow> KVSNonEmp s"
+proof(induction s rule: reach.induct)
+  case (reach_init s)
+  then show ?case
+    by (auto simp add: KVSNonEmp_def tps_defs DS_vl_init_def ep_version_init_def)
+next
+  case (reach_trans s e s')
+  then show ?case
+  proof (induction e)
+    case (RegR x1 x2 x3 x4 x5)
+    then show ?case using reach_trans
+      apply (auto simp add: KVSNonEmp_def tps_trans_defs svr_unchanged_defs)
+      by (metis list_update_nonempty add_to_readerset_def)
+  next
+    case (PrepW x1 x2 x3 x4)
+    then show ?case using reach_trans
+      apply (auto simp add: KVSNonEmp_def tps_trans_defs svr_unchanged_defs)
+      by (metis Nil_is_append_conv)
+  next
+    case (CommitW x1 x2)
+    then show ?case using reach_trans
+      apply (auto simp add: KVSNonEmp_def tps_trans_defs svr_unchanged_defs)
+      by (metis list_update_nonempty commit_in_vl_def)
+  qed (auto simp add: KVSNonEmp_def tps_trans_defs cl_unchanged_defs)
+qed
+
+definition KVS0NonEmp where
+  "KVS0NonEmp s k \<longleftrightarrow> (\<exists>i. i < length (DS (svrs s k)) \<and> \<not>v_is_pending (DS (svrs s k) ! i))"
+
+lemmas KVS0NonEmpI = KVS0NonEmp_def[THEN iffD2, rule_format]
+lemmas KVS0NonEmpE[elim] = KVS0NonEmp_def[THEN iffD1, elim_format, rule_format]
+
+lemma reach_kvs_0_non_emp [simp, intro]: "reach tps s \<Longrightarrow> KVS0NonEmp s k"
+proof(induction s rule: reach.induct)
+  case (reach_init s)
+  then show ?case
+    by (auto simp add: KVS0NonEmp_def tps_defs DS_vl_init_def ep_version_init_def)
+next
+  case (reach_trans s e s')
+  then show ?case
+  proof (induction e)
+    case (RegR x1 x2 x3 x4 x5)
+    then show ?case using reach_trans
+      apply (auto simp add: KVS0NonEmp_def tps_trans_defs svr_unchanged_defs)
+      subgoal for i apply (rule exI[where x=i])
+      by (cases "k = x1"; cases "x4 = i"; auto simp add: add_to_readerset_def).
+  next
+    case (PrepW x1 x2 x3 x4)
+    then show ?case using reach_trans
+      apply (auto simp add: KVS0NonEmp_def tps_trans_defs svr_unchanged_defs)
+      by (metis length_append_singleton less_SucI list_update_append1 list_update_id nth_list_update_eq)
+  next
+    case (CommitW x1 x2)
+    then show ?case using reach_trans
+      apply (auto simp add: KVS0NonEmp_def tps_trans_defs svr_unchanged_defs)
+      subgoal for i kv_map commit_t prep_t y j apply (rule exI[where x=i])
+      by (cases "k = x1"; cases "j = i"; auto simp add: commit_in_vl_def).
+  qed (auto simp add: KVS0NonEmp_def tps_trans_defs cl_unchanged_defs)
+qed
+
+definition KVSSNonEmp where
+  "KVSSNonEmp s \<longleftrightarrow> (\<forall>k. kvs_of_s s k \<noteq> [])"
+
+lemmas KVSSNonEmpI = KVSSNonEmp_def[THEN iffD2, rule_format]
+lemmas KVSSNonEmpE[elim] = KVSSNonEmp_def[THEN iffD1, elim_format, rule_format]
+
+lemma reach_kvs_s_non_emp [simp, intro]:
+  assumes "reach tps s"
+    and "\<And>k. KVS0NonEmp s k"
+  shows "KVSSNonEmp s"
+  using assms
+proof(induction s rule: reach.induct)
+  case (reach_init s)
+  then show ?case
+    by (auto simp add: KVSSNonEmp_def kvs_of_s_def DS_vl_init_def ep_version_init_def get_state_defs
+        tps_defs)
+next
+  case (reach_trans s e s')
+  then show ?case
+    by (induction e; auto simp add: KVSSNonEmp_def KVS0NonEmp_def tps_trans_defs kvs_of_s_def
+        get_state_defs unchanged_defs; metis (lifting) empty_filter_conv nth_mem)
+qed
+
+\<comment> \<open>Invariant about future and past transactions svrs\<close>
+
+definition FutureTIDInv where
+  "FutureTIDInv s cl \<longleftrightarrow> (\<forall>n k. n > txn_sn (cls s cl) \<longrightarrow> wtxn_state (svrs s k) (Tn_cl n cl) = Ready)"
+
+lemmas FutureTIDInvI = FutureTIDInv_def[THEN iffD2, rule_format]
+lemmas FutureTIDInvE[elim] = FutureTIDInv_def[THEN iffD1, elim_format, rule_format]
+
+lemma reach_tidfuturekm [simp, dest]: "reach tps s \<Longrightarrow> FutureTIDInv s cl"
+proof(induction s arbitrary: cl rule: reach.induct)
+  case (reach_init s)
+  then show ?case
+  by (auto simp add: FutureTIDInv_def tps_defs tid_match_def)
+next
+  case (reach_trans s e s')
+  then show ?case 
+  proof (cases e)
+    case (RInvoke x11 x12)
+    then show ?thesis using reach_trans
+      by (auto simp add: tps_trans_defs cl_unchanged_defs tid_match_def FutureTIDInv_def, metis)
+  next
+    case (Read x21 x22 x23)
+    then show ?thesis using reach_trans
+      by (auto simp add: tps_trans_defs cl_unchanged_defs tid_match_def FutureTIDInv_def, metis)
+  next
+    case (RDone x31 x32 x33 x34)
+    then show ?thesis using reach_trans
+      apply (auto simp add: tps_trans_defs cl_unchanged_defs tid_match_def FutureTIDInv_def)
+      by (metis Suc_lessD)
+  next
+    case (WInvoke x41 x42)
+    then show ?thesis using reach_trans
+      by (auto simp add: tps_trans_defs cl_unchanged_defs tid_match_def FutureTIDInv_def, metis)
+  next
+    case (WCommit x51 x52 x53 x54 x55)
+    then show ?thesis using reach_trans
+      apply (auto simp add: tps_trans_defs cl_unchanged_defs tid_match_def FutureTIDInv_def)
+      by (metis (lifting))
+  next
+    case (WDone x6)
+    then show ?thesis  using reach_trans
+      apply (auto simp add: tps_trans_defs cl_unchanged_defs tid_match_def FutureTIDInv_def)
+      by (metis Suc_lessD)
+  next
+    case (RegR x71 x72 x73 x74 x75)
+    then show ?thesis using reach_trans
+      by (auto simp add: tps_trans_defs svr_unchanged_defs tid_match_def FutureTIDInv_def, metis)
+  next
+    case (PrepW x81 x82 x83 x84)
+    then show ?thesis using reach_trans
+      apply (auto simp add: tps_trans_defs svr_unchanged_defs tid_match_def FutureTIDInv_def)
+      by (metis get_cl_txn.simps get_sn_txn.simps nat_neq_iff)
+  next
+    case (CommitW x91 x92)
+    then show ?thesis  using reach_trans
+      apply (auto simp add: tps_trans_defs svr_unchanged_defs tid_match_def FutureTIDInv_def)
+      by (metis state_wtxn.distinct(1))
+  qed simp
+qed
+
+definition PastTIDInv where
+  "PastTIDInv s cl \<longleftrightarrow> (\<forall>n k. n < txn_sn (cls s cl) \<longrightarrow> wtxn_state (svrs s k) (Tn_cl n cl) \<in> {Ready, Commit})"
+
+lemmas PastTIDInvI = PastTIDInv_def[THEN iffD2, rule_format]
+lemmas PastTIDInvE[elim] = PastTIDInv_def[THEN iffD1, elim_format, rule_format]
+
+lemma reach_tidpastkm [simp, dest]: "reach tps s \<Longrightarrow> PastTIDInv s cl"
+proof(induction s arbitrary: cl rule: reach.induct)
+  case (reach_init s)
+  then show ?case
+  by (auto simp add: PastTIDInv_def tps_defs tid_match_def)
+next
+  case (reach_trans s e s')
+  then show ?case 
+  proof (cases e)
+    case (RInvoke x11 x12)
+    then show ?thesis using reach_trans
+      by (auto simp add: tps_trans_defs cl_unchanged_defs tid_match_def PastTIDInv_def, metis)
+  next
+    case (Read x21 x22 x23)
+    then show ?thesis using reach_trans
+      by (auto simp add: tps_trans_defs cl_unchanged_defs tid_match_def PastTIDInv_def, metis)
+  next
+    case (RDone x31 x32 x33 x34)
+    then show ?thesis using reach_trans
+      apply (auto simp add: tps_trans_defs cl_unchanged_defs tid_match_def PastTIDInv_def) sorry
+  next
+    case (WInvoke x41 x42)
+    then show ?thesis using reach_trans
+      by (auto simp add: tps_trans_defs cl_unchanged_defs tid_match_def PastTIDInv_def, metis)
+  next
+    case (WCommit x51 x52 x53 x54 x55)
+    then show ?thesis using reach_trans
+      apply (auto simp add: tps_trans_defs cl_unchanged_defs tid_match_def PastTIDInv_def)
+      by (metis (lifting))
+  next
+    case (WDone x6)
+    then show ?thesis using reach_trans
+      apply (auto simp add: tps_trans_defs cl_unchanged_defs tid_match_def PastTIDInv_def) sorry
+  next
+    case (RegR x71 x72 x73 x74 x75)
+    then show ?thesis using reach_trans
+      by (auto simp add: tps_trans_defs svr_unchanged_defs tid_match_def PastTIDInv_def, metis)
+  next
+    case (PrepW x81 x82 x83 x84)
+    then show ?thesis using reach_trans
+      apply (auto simp add: tps_trans_defs svr_unchanged_defs tid_match_def PastTIDInv_def)
+      by (metis get_cl_txn.simps get_sn_txn.simps nat_neq_iff)
+  next
+    case (CommitW x91 x92)
+    then show ?thesis using reach_trans
+      by (auto simp add: tps_trans_defs svr_unchanged_defs tid_match_def PastTIDInv_def, metis)
+  qed simp
+qed
+
+lemma other_sn_idle:  
+  assumes "FutureTIDInv s cl" and "PastTIDInv s cl"
+    and "get_cl_txn t = cl" and "get_sn_txn t \<noteq> txn_sn (cls s cl)"
+  shows "\<And>k. wtxn_state (svrs s k) t \<in> {Ready, Commit}"
+  using assms
+  apply (auto simp add: FutureTIDInv_def PastTIDInv_def)
+  apply (cases "get_sn_txn t > txn_sn (cls s cl)")
+  apply (metis get_cl_txn.elims get_sn_txn.simps)
+  by (metis get_cl_txn.elims get_sn_txn.simps linorder_cases)
+
+abbreviation not_committing_ev where
+  "not_committing_ev e \<equiv> \<forall>cl kv_map cts sn u. e \<noteq> RDone cl kv_map sn u \<and> e \<noteq> WCommit cl kv_map cts sn u"
+
+abbreviation invariant_list_kvs where
+  "invariant_list_kvs s \<equiv> \<forall>cl k. FutureTIDInv s cl \<and> PastTIDInv s cl \<and> KVSNonEmp s \<and> KVS0NonEmp s k"
+
+abbreviation invariant_list where
+  "invariant_list s \<equiv> invariant_list_kvs s"
+                                                               
+subsection \<open>Refinement Proof\<close>
+
+(*need to add an invariant t is not in the v_readerset in the beginning of the transaction*)
+lemma pending_rtxn_inv:
+  assumes "\<forall>keys kv_map. txn_state (cls s cl) \<noteq> RtxnInProg keys kv_map"
+    and "\<forall>keys kv_map. txn_state (cls s' cl) \<noteq> RtxnInProg keys kv_map"
+    and "\<forall>cl'. cl' \<noteq> cl \<longrightarrow> cls s' cl' = cls s cl'"
+  shows "pending_rtxn s' t = pending_rtxn s t"
+  using assms
+  apply (auto simp add: pending_rtxn_def)oops
+
+lemma pending_wtxn_inv:
+  assumes "\<forall>kv_map. txn_state (cls s cl) \<noteq> WtxnPrep kv_map"
+    and "\<forall>kv_map. txn_state (cls s' cl) \<noteq> WtxnPrep kv_map"
+    and "\<forall>cl'. cl' \<noteq> cl \<longrightarrow> cls s' cl' = cls s cl'"
+  shows "pending_wtxn s' t = pending_wtxn s t"
+  using assms
+  by (auto simp add: pending_wtxn_def split: txid.split txid0.split)
+
+lemma kvs_of_s_inv:
+  assumes "state_trans s e s'"
+    and "invariant_list_kvs s"
+    and "not_committing_ev e"
+  shows "kvs_of_s s' = kvs_of_s s"
+  using assms
+  proof (induction e)
+    case (RInvoke x1 x2)
+    then have "\<And>v. get_ver_committed_rd s' v = get_ver_committed_rd s v"
+      apply (auto simp add: tps_trans_defs get_ver_committed_rd_def) sorry
+    then show ?case using RInvoke reach_trans pending_wtxn_inv[of s x1 s']
+      by (auto simp add: tps_trans_defs kvs_of_s_def get_state_defs cl_unchanged_defs)
+  next
+    case (Read x1 x2 x3)
+    then show ?case sorry
+  next
+    case (WInvoke x1 x2)
+    then show ?case sorry
+  next
+    case (WDone x)
+    then show ?case sorry
+  next
+    case (RegR x1 x2 x3 x4 x5)
+    then show ?case sorry
+  next
+    case (PrepW x1 x2 x3 x4)
+    then show ?case sorry
+  next
+    case (CommitW x1 x2)
+    then show ?case sorry
+  qed auto
+
+lemma tm_view_inv:
+  assumes "state_trans s e s'"
+    and "not_committing_ev e"
+  shows "cl_view (cls s' cl) = cl_view (cls s cl)"
+  using assms by (induction e) (auto simp add: tps_trans_defs unchanged_defs dest!:eq_for_all_cl)
+
+lemma tps_refines_et_es: "tps \<sqsubseteq>\<^sub>med ET_CC.ET_ES"
+proof (intro simulate_ES_fun_with_invariant[where I="\<lambda>s. invariant_list s"])
+  fix gs0 :: "'v state"
+  assume p: "init tps gs0"
+  then show "init ET_CC.ET_ES (sim gs0)"
+    by (auto simp add: ET_CC.ET_ES_defs tps_defs sim_defs DS_vl_init_def ep_version_init_def
+        get_state_defs kvs_init_def v_list_init_def version_init_def)
+next
+  fix gs a and gs' :: "'v state"
+  assume p: "tps: gs\<midarrow>a\<rightarrow> gs'" and inv: "invariant_list gs"
+  then show "ET_CC.ET_ES: sim gs\<midarrow>med a\<rightarrow> sim gs'"
+  using kvs_of_s_inv[of gs a gs'] tm_view_inv[of gs a gs']
+  proof (induction a)
+    case (RDone cl kv_map sn u)
+    then show ?case using p apply simp
+      apply (auto simp add: read_done_def cl_unchanged_defs sim_def)
+      subgoal sorry
+      subgoal apply (auto simp add: fp_property_def view_snapshot_def)
+        subgoal for k y sorry
+        done
+      done
+  next
+    case (WCommit cl kv_map cts sn u)
+    then show ?case using p apply simp
+      apply (auto simp add: write_commit_def cl_unchanged_defs sim_def fp_property_def)
+      sorry
+  qed (auto simp add: sim_defs)
+qed simp
+
+end
