txn-data-consistency/Serializable_2PC_2PL_Invariants.thy
@@ -1,0 +1,433 @@
+section \<open>2PL+2PC Refinement Proof Invariants (and important lemmas)\<close>
+
+theory Serializable_2PC_2PL_Invariants
+  imports Serializable_2PC_2PL
+begin
+
+\<comment> \<open>Invariant about future and past transactions kms\<close>
+
+definition TIDFutureKm where
+  "TIDFutureKm s cl \<longleftrightarrow> (\<forall>n k. n > tm_sn (tm s cl) \<longrightarrow> km_status (kms s k) (Tn_cl n cl) = working)"
+
+definition TIDPastKm where
+  "TIDPastKm s cl \<longleftrightarrow> (\<forall>n k. n < tm_sn (tm s cl) \<longrightarrow> km_status (kms s k) (Tn_cl n cl) \<in> {committed, aborted})"
+
+lemma other_sn_idle:  
+  assumes "TIDFutureKm s cl" and "TIDPastKm s cl"
+    and "get_cl_txn t = cl" and "get_sn_txn t \<noteq> tm_sn (tm s cl)"
+  shows "\<And>k. km_status (kms s k) t \<in> {working, committed, aborted}"
+  oops
+
+\<comment> \<open>Lock Invariants\<close>
+
+definition RLockInv where
+  "RLockInv s k \<longleftrightarrow> (\<forall>t. km_status (kms s k) t = read_lock \<longrightarrow> (\<forall>t. km_status (kms s k) t \<noteq> write_lock))"
+
+definition WLockInv where
+  "WLockInv s k \<longleftrightarrow> (\<forall>t. km_status (kms s k) t \<noteq> write_lock) \<or> (\<exists>! t. km_status (kms s k) t = write_lock)"
+
+\<comment> \<open>Invariants for fingerprint, knowing the lock (km status)\<close>
+
+definition RLockFpInv where
+  "RLockFpInv s k \<longleftrightarrow> (\<forall>t. km_status (kms s k) t = read_lock \<longrightarrow>
+    km_key_fp (kms s k) t W = None \<and>
+    km_key_fp (kms s k) t R \<noteq> None)"
+
+definition WLockFpInv where
+  "WLockFpInv s k \<longleftrightarrow> (\<forall>t. km_status (kms s k) t = write_lock \<longrightarrow> km_key_fp (kms s k) t W \<noteq> None)"
+
+definition NoLockFpInv where
+  "NoLockFpInv s k \<longleftrightarrow> (\<forall>t. km_status (kms s k) t = no_lock \<longrightarrow>
+    km_key_fp (kms s k) t W = None \<and>
+    km_key_fp (kms s k) t R = None)"
+
+\<comment> \<open>Invariants about kv store\<close>
+definition KVSNonEmp where
+  "KVSNonEmp s \<longleftrightarrow> (\<forall>k. km_vl (kms s k) \<noteq> [])"
+
+definition KVSGSNonEmp where
+  "KVSGSNonEmp s \<longleftrightarrow> (\<forall>k. kvs_of_gs s k \<noteq> [])"
+
+definition KVSLen where
+  "KVSLen s cl \<longleftrightarrow> (\<forall>k. length (km_vl (kms s k)) \<le> length (kvs_of_gs s k))"
+
+subsubsection \<open>Lemmas for kvs_of_gs changing by different events\<close>
+
+lemma kvs_of_gs_km_inv:
+  assumes "WLockInv s k" and "RLockInv s k"
+    and "(\<forall>t. km_status (kms s k) t \<noteq> write_lock) \<or> 
+              km_status (kms s' k) t \<noteq> write_lock"
+    and "tm_status (tm s (get_cl_txn t)) \<noteq> tm_committed"
+    and "\<And>k. km_vl (kms s' k) = km_vl (kms s k)"
+    and "tm_km_k'_t'_unchanged k s s' t"
+  shows "kvs_of_gs s' = kvs_of_gs s"
+  oops
+
+lemma kvs_of_gs_tm_inv:
+  assumes "TIDFutureKm s cl" and "TIDPastKm s cl"
+    and "tm_status (tm s cl) \<noteq> tm_committed \<or>
+         (\<forall>k. km_status (kms s k) (get_txn_cl cl s) = committed)"
+    and "tm_status (tm s' cl) \<noteq> tm_committed"
+    and "km_tm_cl'_unchanged cl s s'"
+  shows "kvs_of_gs s' = kvs_of_gs s"
+  oops
+
+lemma update_kv_all_tm_commit_no_lock_inv:
+  assumes "TIDPastKm s cl" and "TIDFutureKm s cl"
+    and "tm_status (tm s cl) = tm_prepared"
+    and "tm_status (tm s' cl) = tm_committed"
+    and "other_insts_unchanged cl (tm s) (tm s')"
+    and "km_status (kms s k) (get_txn_cl cl s) = no_lock"
+  shows "update_kv_all_txn (\<lambda>t. tm_status (tm s' (get_cl_txn t))) (km_status (kms s k))
+          (km_key_fp (kms s k)) (km_vl (kms s k)) =
+         update_kv_all_txn (\<lambda>t. tm_status (tm s (get_cl_txn t))) (km_status (kms s k))
+          (km_key_fp (kms s k)) (km_vl (kms s k))"
+  oops
+
+(*All events*)
+abbreviation not_tm_commit where
+  "not_tm_commit e \<equiv> \<forall>cl sn u F. e \<noteq> TM_Commit cl sn u F"
+
+abbreviation invariant_list_kvs where
+  "invariant_list_kvs s \<equiv> \<forall>cl k. TIDFutureKm s cl \<and> TIDPastKm s cl \<and> RLockInv s k \<and> WLockInv s k \<and>
+                        RLockFpInv s k \<and> NoLockFpInv s k \<and> KVSNonEmp s"
+
+lemma kvs_of_gs_inv:
+  assumes "gs_trans s e s'"
+    and "invariant_list_kvs s"
+    and "not_tm_commit e"
+  shows "kvs_of_gs s' = kvs_of_gs s"
+  oops
+
+\<comment> \<open>More specific lemmas about TM commit\<close>
+lemma kvs_of_gs_commit_length_increasing:
+  assumes "tm_status (tm s cl) = tm_prepared"
+    and "tm_status (tm s' cl) = tm_committed"
+    and "km_tm_cl'_unchanged cl s s'"
+  shows "length (kvs_of_gs s k) \<le> length (kvs_of_gs s' k)"
+  oops
+
+lemma kvs_of_gs_length_increasing:
+  assumes "gs_trans s e s'"
+    and "invariant_list_kvs s"
+  shows "\<And>k. length (kvs_of_gs s k) \<le> length (kvs_of_gs s' k)"
+  oops
+
+\<comment> \<open>Fingerprint content invariant and Lemmas for proving the fp_property\<close>
+
+lemma km_vl_read_lock_commit_eq_length:
+  assumes "RLockFpInv s k"
+    and "km_status (kms s k) t = read_lock"
+    and "km_vl (kms s' k) =
+          update_kv_key t (km_key_fp (kms s k) t) (full_view (km_vl (kms s k))) (km_vl (kms s k))"
+  shows "length (km_vl (kms s' k)) = length (km_vl (kms s k))"
+  oops
+
+definition RLockFpContentInv where
+  "RLockFpContentInv s k \<longleftrightarrow> (\<forall>t. km_status (kms s k) t = read_lock \<longrightarrow>
+    km_key_fp (kms s k) t R =
+      Some (v_value (last_version (km_vl (kms s k)) (full_view (km_vl (kms s k))))))"
+
+definition WLockFpContentInv where
+  "WLockFpContentInv s k \<longleftrightarrow> (\<forall>t. km_status (kms s k) t = write_lock \<longrightarrow>
+    km_key_fp (kms s k) t R = None \<or>
+    km_key_fp (kms s k) t R =
+      Some (v_value (last_version (km_vl (kms s k)) (full_view (km_vl (kms s k))))))"
+
+lemma km_vl_kvs_eq_length:
+  assumes "WLockInv s k" and "RLockInv s k"
+    and "tm_status (tm s cl) = tm_prepared"
+    and "km_status (kms s k) (get_txn_cl cl s) \<in> {read_lock, write_lock}"
+  shows "length (kvs_of_gs s k) = length (km_vl (kms s k))"
+  oops
+
+\<comment> \<open>Lemmas for view growth after commit\<close>
+
+lemma committed_kvs_view_grows:
+  assumes "tm_status (tm s cl) = tm_prepared"
+    and "tm_status (tm s' cl) = tm_committed"
+    and "km_tm_cl'_unchanged cl s s'"
+  shows "(\<lambda>k. full_view (kvs_of_gs s k)) \<sqsubseteq> (\<lambda>k. full_view (kvs_of_gs s' k))"
+  oops
+  
+lemma updated_vl_view_grows:
+  assumes "km_vl (kms s' k) =
+    update_kv_key t (km_key_fp (kms s k) t) (full_view (km_vl (kms s k))) (km_vl (kms s k))"
+    and "other_insts_unchanged k (kms s) (kms s')"
+  shows "(\<lambda>k. full_view (km_vl (kms s k))) \<sqsubseteq> (\<lambda>k. full_view (km_vl (kms s' k)))"
+  oops
+
+lemma tm_view_inv:
+  assumes "gs_trans s e s'"
+    and "not_tm_commit e"
+  shows "tm_view (tm s' cl) = tm_view (tm s cl)"
+  oops
+
+definition TMFullView where
+  "TMFullView s cl \<longleftrightarrow> tm_view (tm s cl) \<sqsubseteq> (\<lambda>k. full_view (kvs_of_gs s k))"
+
+\<comment> \<open>TM_commit updating kv\<close>
+
+lemma kvs_of_gs_tm_commit:
+  assumes "TIDFutureKm s cl" and "TIDPastKm s cl"
+    and "WLockInv s k" and "WLockFpInv s k"
+    and "RLockInv s k" and "RLockFpInv s k"
+    and "NoLockFpInv s k" and "KVSNonEmp s"
+    and "tm_status (tm s cl) = tm_prepared"
+    and "km_status (kms s k) (get_txn_cl cl s) \<in> {read_lock, write_lock, no_lock}"
+    and "tm_status (tm s' cl) = tm_committed"
+    and "other_insts_unchanged cl (tm s) (tm s')"
+  shows "update_kv_all_txn (\<lambda>t. tm_status (tm s' (get_cl_txn t))) (km_status (kms s k))
+          (km_key_fp (kms s k)) (km_vl (kms s k)) =
+    update_kv_key (get_txn_cl cl s) (km_key_fp (kms s k) (get_txn_cl cl s))
+      (full_view (update_kv_all_txn (\<lambda>t. tm_status (tm s (get_cl_txn t))) (km_status (kms s k))
+        (km_key_fp (kms s k)) (km_vl (kms s k))))
+      (update_kv_all_txn (\<lambda>t. tm_status (tm s (get_cl_txn t))) (km_status (kms s k))
+        (km_key_fp (kms s k)) (km_vl (kms s k)))"
+  oops
+
+\<comment> \<open>Lemmas for showing transaction id freshness\<close>
+
+lemma get_sqns_other_cl_inv:
+  assumes "TIDFutureKm s cl" and "TIDPastKm s cl"
+    and "\<And>k. WLockInv s k" and "\<And>k. WLockFpInv s k"
+    and "\<And>k. RLockInv s k" and "\<And>k. RLockFpInv s k"
+    and "\<And>k. NoLockFpInv s k" and "KVSNonEmp s"
+    and "tm_status (tm s cl) = tm_prepared"
+    and "tm_status (tm s' cl) = tm_committed"
+    and "\<And>k. km_status (kms s k) (get_txn_cl cl s) = read_lock \<or>
+             km_status (kms s k) (get_txn_cl cl s) = write_lock \<or> 
+             km_status (kms s k) (get_txn_cl cl s) = no_lock"
+    and "km_tm_cl'_unchanged cl s s'"
+    and "cl' \<noteq> cl"
+  shows "get_sqns (kvs_of_gs s') cl' = get_sqns (kvs_of_gs s) cl'"
+  oops
+
+lemma new_t_is_in_writers:
+  assumes "TIDFutureKm s cl" and "TIDPastKm s cl"
+    and "\<And>k. WLockInv s k" and "\<And>k. WLockFpInv s k"
+    and "\<And>k. RLockInv s k" and "\<And>k. RLockFpInv s k"
+    and "\<And>k. NoLockFpInv s k" and "KVSNonEmp s"
+    and "tm_status (tm s cl) = tm_prepared"
+    and "tm_status (tm s' cl) = tm_committed"
+    and "km_status (kms s k) (get_txn_cl cl s) = write_lock"
+    and "other_insts_unchanged cl (tm s) (tm s')"
+    and "kms s' = kms s"
+  shows "vl_writers_sqns (kvs_of_gs s' k) cl = vl_writers_sqns (kvs_of_gs s k) cl \<union> {tm_sn (tm s cl)}"
+  oops
+
+lemma new_t_is_in_writers2:
+  assumes "TIDFutureKm s cl" and "TIDPastKm s cl"
+    and "\<And>k. WLockInv s k" and "\<And>k. WLockFpInv s k"
+    and "\<And>k. RLockInv s k" and "\<And>k. RLockFpInv s k"
+    and "\<And>k. NoLockFpInv s k" and "KVSNonEmp s"
+    and "tm_status (tm s cl) = tm_prepared"
+    and "tm_status (tm s' cl) = tm_committed"
+    and "km_status (kms s k) (get_txn_cl cl s) = read_lock"
+    and "other_insts_unchanged cl (tm s) (tm s')"
+    and "kms s' = kms s"
+  shows "vl_writers_sqns (kvs_of_gs s' k) cl = vl_writers_sqns (kvs_of_gs s k) cl"
+  oops
+
+lemma new_t_is_in_readers:
+  assumes "TIDFutureKm s cl" and "TIDPastKm s cl"
+    and "\<And>k. WLockInv s k" and "\<And>k. WLockFpInv s k"
+    and "\<And>k. RLockInv s k" and "\<And>k. RLockFpInv s k"
+    and "\<And>k. NoLockFpInv s k" and "KVSNonEmp s"
+    and "tm_status (tm s cl) = tm_prepared"
+    and "tm_status (tm s' cl) = tm_committed"
+    and "km_status (kms s k) (get_txn_cl cl s) = read_lock"
+    and "other_insts_unchanged cl (tm s) (tm s')"
+    and "kms s' = kms s"
+  shows "vl_readers_sqns (kvs_of_gs s' k) cl = vl_readers_sqns (kvs_of_gs s k) cl \<union> {tm_sn (tm s cl)}"
+  oops
+
+lemma new_t_is_in_readers2:
+  assumes "TIDFutureKm s cl" and "TIDPastKm s cl"
+    and "\<And>k. WLockInv s k" and "\<And>k. WLockFpInv s k"
+    and "\<And>k. RLockInv s k" and "\<And>k. RLockFpInv s k"
+    and "\<And>k. NoLockFpInv s k" and "KVSNonEmp s"
+    and "tm_status (tm s cl) = tm_prepared"
+    and "tm_status (tm s' cl) = tm_committed"
+    and "km_status (kms s k) (get_txn_cl cl s) = write_lock"
+    and "km_key_fp (kms s k) (get_txn_cl cl s) R \<noteq> None"
+    and "other_insts_unchanged cl (tm s) (tm s')"
+    and "kms s' = kms s"
+  shows "vl_readers_sqns (kvs_of_gs s' k) cl = vl_readers_sqns (kvs_of_gs s k) cl \<union> {tm_sn (tm s cl)}"
+  oops
+
+lemma new_t_is_in_readers3:
+  assumes "TIDFutureKm s cl" and "TIDPastKm s cl"
+    and "\<And>k. WLockInv s k" and "\<And>k. WLockFpInv s k"
+    and "\<And>k. RLockInv s k" and "\<And>k. RLockFpInv s k"
+    and "\<And>k. NoLockFpInv s k" and "KVSNonEmp s"
+    and "tm_status (tm s cl) = tm_prepared"
+    and "tm_status (tm s' cl) = tm_committed"
+    and "km_status (kms s k) (get_txn_cl cl s) = write_lock"
+    and "km_key_fp (kms s k) (get_txn_cl cl s) R = None"
+    and "other_insts_unchanged cl (tm s) (tm s')"
+    and "kms s' = kms s"
+  shows "vl_readers_sqns (kvs_of_gs s' k) cl = vl_readers_sqns (kvs_of_gs s k) cl"
+  oops
+
+lemma kvs_writers_tm_commit_grows:
+  assumes "TIDFutureKm s cl" and "TIDPastKm s cl"
+    and "\<And>k. WLockInv s k" and "\<And>k. WLockFpInv s k"
+    and "\<And>k. RLockInv s k" and "\<And>k. RLockFpInv s k"
+    and "\<And>k. NoLockFpInv s k" and "KVSNonEmp s"
+    and "tm_status (tm s cl) = tm_prepared"
+    and "tm_status (tm s' cl) = tm_committed"
+    and "\<forall>k. km_status (kms s k) (get_txn_cl cl s) \<in> {read_lock, write_lock, no_lock}"
+    and "km_status (kms s k) (get_txn_cl cl s) = write_lock"
+    and "other_insts_unchanged cl (tm s) (tm s')"
+    and "kms s' = kms s"
+  shows "kvs_writers_sqns (kvs_of_gs s') cl = kvs_writers_sqns (kvs_of_gs s) cl \<union> {tm_sn (tm s cl)}"
+  oops
+
+lemma kvs_writers_tm_commit_doesnt_grow:
+  assumes "TIDFutureKm s cl" and "TIDPastKm s cl"
+    and "\<And>k. WLockInv s k" and "\<And>k. WLockFpInv s k"
+    and "\<And>k. RLockInv s k" and "\<And>k. RLockFpInv s k"
+    and "\<And>k. NoLockFpInv s k" and "KVSNonEmp s"
+    and "tm_status (tm s cl) = tm_prepared"
+    and "tm_status (tm s' cl) = tm_committed"
+    and "\<forall>k. km_status (kms s k) (get_txn_cl cl s) \<in> {read_lock, no_lock}"
+    and "other_insts_unchanged cl (tm s) (tm s')"
+    and "kms s' = kms s"
+  shows "kvs_writers_sqns (kvs_of_gs s') cl = kvs_writers_sqns (kvs_of_gs s) cl"
+  oops
+
+lemma kvs_readers_sqns_tm_commit_grows:
+  assumes "TIDFutureKm s cl" and "TIDPastKm s cl"
+    and "\<And>k. WLockInv s k" and "\<And>k. WLockFpInv s k"
+    and "\<And>k. RLockInv s k" and "\<And>k. RLockFpInv s k"
+    and "\<And>k. NoLockFpInv s k" and "KVSNonEmp s"
+    and "tm_status (tm s cl) = tm_prepared"
+    and "tm_status (tm s' cl) = tm_committed"
+    and "\<forall>k. km_status (kms s k) (get_txn_cl cl s) \<in> {read_lock, write_lock, no_lock}"
+    and "km_status (kms s k) (get_txn_cl cl s) = read_lock \<or>
+         (km_status (kms s k) (get_txn_cl cl s) = write_lock \<and>
+          km_key_fp (kms s k) (get_txn_cl cl s) R \<noteq> None)"
+    and "other_insts_unchanged cl (tm s) (tm s')"
+    and "kms s' = kms s"
+  shows "kvs_readers_sqns (kvs_of_gs s') cl = kvs_readers_sqns (kvs_of_gs s) cl \<union> {tm_sn (tm s cl)}"
+  oops
+
+lemma kvs_readers_sqns_tm_commit_doesnt_grow:
+  assumes "TIDFutureKm s cl" and "TIDPastKm s cl"
+    and "\<And>k. WLockInv s k" and "\<And>k. WLockFpInv s k"
+    and "\<And>k. RLockInv s k" and "\<And>k. RLockFpInv s k"
+    and "\<And>k. NoLockFpInv s k" and "KVSNonEmp s"
+    and "tm_status (tm s cl) = tm_prepared"
+    and "tm_status (tm s' cl) = tm_committed"
+    and "\<forall>k. km_status (kms s k) (get_txn_cl cl s) \<in> {write_lock, no_lock}"
+    and "\<forall>k. km_status (kms s k) (get_txn_cl cl s) \<noteq> write_lock \<or>
+             km_key_fp (kms s k) (get_txn_cl cl s) R = None"
+    and "other_insts_unchanged cl (tm s) (tm s')"
+    and "kms s' = kms s"
+  shows "kvs_readers_sqns (kvs_of_gs s') cl = kvs_readers_sqns (kvs_of_gs s) cl"
+  oops
+
+lemma get_sqns_tm_commit_grows:
+  assumes "TIDFutureKm s cl" and "TIDPastKm s cl"
+    and "\<And>k. WLockInv s k" and "\<And>k. WLockFpInv s k"
+    and "\<And>k. RLockInv s k" and "\<And>k. RLockFpInv s k"
+    and "\<And>k. NoLockFpInv s k" and "KVSNonEmp s"
+    and "tm_status (tm s cl) = tm_prepared"
+    and "tm_status (tm s' cl) = tm_committed"
+    and "\<And>k. km_status (kms s k) (get_txn_cl cl s) \<in> {read_lock, write_lock, no_lock}"
+    and "other_insts_unchanged cl (tm s) (tm s')"
+    and "kms s' = kms s"
+  shows "get_sqns (kvs_of_gs s') cl =
+         (if \<forall>k. km_status (kms s k) (get_txn_cl cl s) = no_lock then
+          get_sqns (kvs_of_gs s) cl else
+          get_sqns (kvs_of_gs s) cl \<union> {tm_sn (tm s cl)})"
+  oops
+
+definition SqnInv where
+  "SqnInv s cl \<longleftrightarrow>
+    (tm_status (tm s cl) \<noteq> tm_committed \<longrightarrow> (\<forall>m \<in> get_sqns (kvs_of_gs s) cl. m < tm_sn (tm s cl))) \<and>
+    (tm_status (tm s cl) = tm_committed \<longrightarrow> (\<forall>m \<in> get_sqns (kvs_of_gs s) cl. m \<le> tm_sn (tm s cl)))"
+
+
+\<comment> \<open>Lemmas for proving view wellformedness of tm_view\<close>
+
+lemma kvs_of_gs_version_order:
+  assumes "TIDPastKm s cl" and "TIDFutureKm s cl" and "WLockInv s k" and "RLockInv s k" and "KVSNonEmp s"
+    and "i \<in> full_view (kvs_of_gs s k)"
+    and "tm_status (tm s cl) = tm_prepared"
+    and "tm_status (tm s' cl) = tm_committed"
+    and "km_status (kms s k) (get_txn_cl cl s) \<in> {read_lock, write_lock, no_lock}"
+    and "km_tm_cl'_unchanged cl s s'"
+  shows "kvs_of_gs s k ! i \<sqsubseteq>\<^sub>v\<^sub>e\<^sub>r kvs_of_gs s' k ! i"
+  oops
+
+lemma new_version_index:
+  assumes "TIDPastKm s cl" and "TIDFutureKm s cl"
+    and "WLockInv s k" and "KVSNonEmp s"
+    and "tm_status (tm s cl) = tm_prepared"
+    and "tm_status (tm s' cl) = tm_committed"
+    and "km_status (kms s k) (get_txn_cl cl s) = write_lock"
+    and "other_insts_unchanged cl (tm s) (tm s')"
+    and "i \<in> full_view (update_kv_all_txn (\<lambda>t. tm_status (tm s' (get_cl_txn t)))
+    (km_status (kms s k)) (km_key_fp (kms s k)) (km_vl (kms s k)))"
+    and "i \<notin> full_view (update_kv_all_txn (\<lambda>t. tm_status (tm s (get_cl_txn t)))
+    (km_status (kms s k)) (km_key_fp (kms s k)) (km_vl (kms s k)))"
+  shows "i = length (km_vl (kms s k))"
+  oops
+
+lemma t_is_fresh:
+  assumes "SqnInv s cl"
+    and "tm_status (tm s cl) = tm_prepared"
+  shows "get_txn_cl cl s \<in> next_txids (kvs_of_gs s) cl"
+  oops
+
+lemma kvs_of_gs_view_atomic:
+  assumes "TIDPastKm s cl" and "TIDFutureKm s cl"
+    and "\<And>k. WLockInv s k" and "\<And>k. WLockFpInv s k"
+    and "\<And>k. RLockInv s k" and "\<And>k. NoLockFpInv s k"
+    and "SqnInv s cl" and "KVSNonEmp s"
+    and "tm_status (tm s cl) = tm_prepared"
+    and "tm_status (tm s' cl) = tm_committed"
+    and "\<forall>k. km_status (kms s k) (get_txn_cl cl s) \<in> {read_lock, write_lock, no_lock}"
+    and "km_tm_cl'_unchanged cl s s'"
+  shows "view_atomic (kvs_of_gs s') (\<lambda>k. full_view (kvs_of_gs s k))"
+  oops
+
+lemma reach_kvs_expands [simp, intro]:
+  assumes "reach tps s" and "gs_trans s e s'"
+    and "\<And>cl. TIDFutureKm s cl" and "\<And>cl. TIDPastKm s cl"
+    and "\<And>k. RLockInv s k" and "\<And>k. WLockInv s k"
+    and "\<And>k. RLockFpInv s k" and "\<And>k. NoLockFpInv s k"
+    and "KVSNonEmp s" and "KVSLen s cl"
+  shows "kvs_of_gs s \<sqsubseteq>\<^sub>k\<^sub>v\<^sub>s kvs_of_gs s'"
+  oops
+
+definition KVSView where
+  "KVSView s cl \<longleftrightarrow> view_wellformed (kvs_of_gs s) (tm_view (tm s cl))"
+
+\<comment> \<open>CanCommit\<close>
+
+lemma writers_visible:
+  assumes "u = (\<lambda>k. full_view (K k))"
+  shows "visTx K u = kvs_writers K"
+  oops
+
+lemma WW_writers_id_helper:
+  assumes "(x, v_writer x') \<in> {(xa, x). \<exists>xb i.
+            i \<in> full_view (K xb) \<and>
+            (\<exists>i'. i' \<in> full_view (K xb) \<and>
+              x = v_writer (K xb ! i) \<and> xa = v_writer (K xb ! i') \<and> i < i')}\<^sup>* "
+    and "x' \<in> set (K k)"
+  shows "\<exists>xa. x \<in> v_writer ` set (K xa)"
+  oops
+
+lemma WW_writers_id:
+  "(((\<Union> (range (WW K)))\<inverse>)\<^sup>*)\<inverse> `` kvs_writers K = kvs_writers K"
+  oops
+
+lemma full_view_satisfies_ET_SER_canCommit:
+  "u = (\<lambda>k. full_view (K k)) \<Longrightarrow> ET_SER.canCommit K u F"
+  oops
+
+end
